src/cbor/pulse/raw/everparse/CBOR.Pulse.Raw.EverParse.Nondet.fst
@@ -68,6 +68,241 @@ pts_to_serialized (serialize_nlist n1 serialize_raw_data_item) l1 #p1 gl1 **
       )
     )
 
+let pts_to_serialized_nlist_raw_data_item_head_header'_post_children
+  (n: pos)
+  (va: LowParse.Spec.VCList.nlist n raw_data_item)
+  (h: header) (v': (header & (leaf_content h & (nlist (remaining_data_items_header h) raw_data_item & nlist (n - 1)  raw_data_item  ))))
+: Lemma
+  (requires
+    pts_to_serialized_nlist_raw_data_item_head_header'_post n va h v'
+  )
+  (ensures
+    (fst (snd (snd v')) <: list raw_data_item) == begin match List.Tot.hd va with
+    | Array _ v -> v
+    | Map _ v -> CBOR.Spec.Util.list_of_pair_list v
+    | Tagged _ v -> [v]
+    | _ -> []
+    end
+  )
+= // assert (synth_raw_data_item_from_alt (synth_raw_data_item_from_alt_recip (List.Tot.hd va)) == List.Tot.hd va);
+  ()
+
+let check_equiv_head
+  (a1 a2: raw_data_item)
+: Tot bool
+= 
+      match a1, a2 with
+      | Int64 ty1 v1, Int64 ty2 v2 ->
+        ty1 = ty2 &&
+        v1.value = v2.value
+      | Simple v1, Simple v2 ->
+        v1 = v2
+      | String ty1 _ s1, String ty2 _ s2 ->
+        ty1 = ty2 &&
+        s1 = s2
+      | Tagged tag1 b1, Tagged tag2 b2 ->
+        tag1.value = tag2.value
+      | Array len1 ar1, Array len2 ar2 ->
+        len1.value = len2.value
+      | _ -> false
+
+let check_equiv_head_correct_pre
+  (gl1: list raw_data_item)
+  (gl2: list raw_data_item)
+  (equiv: ((x1: raw_data_item) -> (x2: raw_data_item { raw_data_item_size x1 + raw_data_item_size x2 <= list_sum raw_data_item_size gl1 + list_sum raw_data_item_size gl2 }) -> option bool))
+: Tot prop
+=
+    List.Tot.length gl1 == List.Tot.length gl2 /\
+    Cons? gl1 /\ Cons? gl2 /\ (
+    let a1 = List.Tot.hd gl1 in
+    let a2 = List.Tot.hd gl2 in
+    let gc1 = dsnd (dfst (synth_raw_data_item_from_alt_recip a1)) in
+    let gc2 = dsnd (dfst (synth_raw_data_item_from_alt_recip a2)) in
+    let h1 = get_raw_data_item_header a1 in
+    let h2 = get_raw_data_item_header a2 in
+    get_header_major_type h1 == get_header_major_type h2 /\
+    equiv a1 a2 = Some false
+  )
+
+let check_equiv_head_correct_post
+  (gl1: list raw_data_item)
+  (gl2: list raw_data_item)
+  (equiv: ((x1: raw_data_item) -> (x2: raw_data_item { raw_data_item_size x1 + raw_data_item_size x2 <= list_sum raw_data_item_size gl1 + list_sum raw_data_item_size gl2 }) -> option bool))
+: Tot prop
+=
+  check_equiv_head_correct_pre gl1 gl2 equiv /\ (
+    let a1 :: q1 = gl1 in
+    let a2 :: q2 = gl2 in
+    let l1' = dsnd (synth_raw_data_item_from_alt_recip a1) `List.Tot.append` q1 in
+    let l2' = dsnd (synth_raw_data_item_from_alt_recip a2) `List.Tot.append` q2 in
+    (check_equiv_head a1 a2 ==> list_sum raw_data_item_size l1' + list_sum raw_data_item_size l2' <= list_sum raw_data_item_size gl1 + list_sum raw_data_item_size gl2) /\
+    check_equiv_list gl1 gl2 equiv == (if check_equiv_head a1 a2 then check_equiv_list l1' l2' equiv else Some false)
+  )
+
+#push-options "--z3rlimit 32"
+
+let check_equiv_head_correct
+  (gl1: list raw_data_item)
+  (gl2: list raw_data_item)
+  (equiv: ((x1: raw_data_item) -> (x2: raw_data_item { raw_data_item_size x1 + raw_data_item_size x2 <= list_sum raw_data_item_size gl1 + list_sum raw_data_item_size gl2 }) -> option bool))
+  (sq: squash (check_equiv_head_correct_pre gl1 gl2 equiv))
+: Lemma
+  (ensures (
+    check_equiv_head_correct_post gl1 gl2 equiv
+  ))
+=
+  let a1 :: q1 = gl1 in
+  let a2 :: q2 = gl2 in
+  let l1' = dsnd (synth_raw_data_item_from_alt_recip a1) `List.Tot.append` q1 in
+  let l2' = dsnd (synth_raw_data_item_from_alt_recip a2) `List.Tot.append` q2 in
+  raw_data_item_size_eq a1;
+  raw_data_item_size_eq a2;
+  match a1, a2 with
+  | Array len1 ar1, Array len2 ar2 ->
+        list_sum_append raw_data_item_size ar1 q1;
+        list_sum_append raw_data_item_size ar2 q2;
+        ()
+  | _ ->  ()
+
+module U64 = FStar.UInt64
+
+#pop-options
+
+#push-options "--z3rlimit 64"
+
+let pi
+  (h1: header)
+  (mt1: major_type_t)
+  (len: U64.t)
+  (sq: squash (
+      mt1 == get_header_major_type h1 /\
+      (mt1 == cbor_major_type_byte_string \/ mt1 == cbor_major_type_text_string) /\
+      len == argument_as_uint64 (dfst h1) (dsnd h1) 
+  ))
+= 
+  parse_synth  (parse_filter (LowParse.Spec.SeqBytes.parse_lseq_bytes (U64.v len)) (lseq_utf8_correct mt1 _)) (LeafContentSeq #h1 ())
+
+let pi_correct
+  (h1: header)
+  (mt1: major_type_t)
+  (len: U64.t)
+  (sq: squash (
+      mt1 == get_header_major_type h1 /\
+      (mt1 == cbor_major_type_byte_string \/ mt1 == cbor_major_type_text_string) /\
+      len == argument_as_uint64 (dfst h1) (dsnd h1) 
+  ))
+: Lemma
+  (forall b . parse (parse_leaf_content h1) b == parse (pi h1 mt1 len sq) b)
+= ()
+
+let sigma
+  (h1: header)
+  (mt1: major_type_t)
+  (len: U64.t)
+  (sq: squash (
+      mt1 == get_header_major_type h1 /\
+      (mt1 == cbor_major_type_byte_string \/ mt1 == cbor_major_type_text_string) /\
+      len == argument_as_uint64 (dfst h1) (dsnd h1) 
+  ))
+: serializer (pi h1 mt1 len sq)
+= 
+  serialize_synth  #_ #_ #(c: leaf_content h1 {b2t (LeafContentSeq? #h1 c)}) _ (LeafContentSeq #h1 ()) (serialize_filter (LowParse.Spec.SeqBytes.serialize_lseq_bytes (U64.v len)) (lseq_utf8_correct mt1 _)) (LeafContentSeq?.v #h1) ()
+
+// FIXME: WHY WHY WHY do I need to break abstraction here? I can't unfold sigma in pulse.
+let sigma_correct
+  (a1: raw_data_item)
+  (h1: header)
+  (mt1: major_type_t)
+  (len: U64.t)
+  (c1: leaf_content h1)
+  (sq: squash (
+      mt1 == get_header_major_type h1 /\
+      (mt1 == cbor_major_type_byte_string \/ mt1 == cbor_major_type_text_string) /\
+      len == argument_as_uint64 (dfst h1) (dsnd h1) /\
+      h1 == get_raw_data_item_header a1 /\
+      c1 == dsnd (dfst (synth_raw_data_item_from_alt_recip a1))
+  ))
+: Lemma
+  (serialize (sigma h1 mt1 len ()) c1 == String?.v a1)
+= assert (serialize (sigma h1 mt1 len ()) c1 == serialize (serialize_synth #_ #_ #(c: leaf_content h1 {b2t (LeafContentSeq? #h1 c)}) _ (LeafContentSeq #h1 ()) (serialize_filter (LowParse.Spec.SeqBytes.serialize_lseq_bytes (U64.v len)) (lseq_utf8_correct mt1 _)) (LeafContentSeq?.v #h1) ()) c1)
+  ;
+  serialize_synth_eq
+    _ (LeafContentSeq #h1 ()) (serialize_filter (LowParse.Spec.SeqBytes.serialize_lseq_bytes (U64.v len)) (lseq_utf8_correct mt1 _)) (LeafContentSeq?.v #h1) ()
+    c1;
+  assert ((LeafContentSeq?.v c1 <: bytes ) == (String?.v a1 <: bytes));
+  assert (serialize (sigma h1 mt1 len ()) c1 == serialize (serialize_filter (LowParse.Spec.SeqBytes.serialize_lseq_bytes (U64.v len)) (lseq_utf8_correct mt1 _)) (LeafContentSeq?.v #h1 c1));
+  assert (serialize (sigma h1 mt1 len ()) c1 == String?.v a1);
+  ()
+
+inline_for_extraction
+fn impl_check_equiv_head
+  (h1: header)
+  (c1: S.slice byte)
+  (h2: header)
+  (c2: S.slice byte)
+  (#p1: perm)
+  (#gc1: Ghost.erased (leaf_content h1))
+  (#p2: perm)
+  (#gc2: Ghost.erased (leaf_content h2))
+  (a1: Ghost.erased raw_data_item)
+  (a2: Ghost.erased raw_data_item)
+requires
+  pts_to_serialized (serialize_leaf_content h1) c1 #p1 gc1 **
+  pts_to_serialized (serialize_leaf_content h2) c2 #p2 gc2 **
+  pure (
+    h1 == get_raw_data_item_header a1 /\
+    Ghost.reveal gc1 == dsnd (dfst (synth_raw_data_item_from_alt_recip a1)) /\
+    h2 == get_raw_data_item_header a2 /\
+    Ghost.reveal gc2 == dsnd (dfst (synth_raw_data_item_from_alt_recip a2)) /\
+    get_header_major_type h1 == get_header_major_type h2
+  )
+returns res: bool
+ensures
+  pts_to_serialized (serialize_leaf_content h1) c1 #p1 gc1 **
+  pts_to_serialized (serialize_leaf_content h2) c2 #p2 gc2 **
+  pure (
+    res == check_equiv_head a1 a2
+  )
+{
+  let mt1 = get_header_major_type h1;
+  if (mt1 = cbor_major_type_simple_value) {
+    (argument_as_simple_value (dfst h1) (dsnd h1) = argument_as_simple_value (dfst h2) (dsnd h2))
+  } else {
+    let len = argument_as_uint64 (dfst h1) (dsnd h1);
+    if (len <> argument_as_uint64 (dfst h2) (dsnd h2)) {
+      false
+    } else if (mt1 = cbor_major_type_byte_string || mt1 = cbor_major_type_text_string) {
+      pi_correct h1 mt1 len ();
+      pts_to_serialized_ext_trade
+        (serialize_leaf_content h1)
+        (sigma h1 mt1 len ())
+        c1;
+      sigma_correct a1 h1 mt1 len gc1 ();
+      pts_to_serialized_elim_trade
+        (sigma h1 mt1 len ())
+        c1;
+      Trade.trans _ _ (pts_to_serialized (serialize_leaf_content h1) c1 #p1 gc1);
+      pi_correct h2 mt1 len ();
+      pts_to_serialized_ext_trade
+        (serialize_leaf_content h2)
+        (sigma h2 mt1 len ())
+        c2;
+      sigma_correct a2 h2 mt1 len gc2 ();
+      pts_to_serialized_elim_trade
+        (sigma h2 mt1 len ())
+        c2;
+      Trade.trans _ _ (pts_to_serialized (serialize_leaf_content h2) c2 #p2 gc2);
+      CBOR.Spec.Raw.Format.bytes_lex_compare_equal (String?.v a1) (String?.v a2);
+      let cmp = CBOR.Pulse.Raw.Compare.Bytes.lex_compare_bytes c1 c2;
+      Trade.elim _ (pts_to_serialized (serialize_leaf_content h1) c1 #p1 gc1);
+      Trade.elim _ (pts_to_serialized (serialize_leaf_content h2) c2 #p2 gc2);
+      (cmp = 0s)
+    } else {
+       (mt1 <> cbor_major_type_map)
+    }
+  }
+}
+
 inline_for_extraction
 fn impl_check_equiv_list
   (n1: SZ.t)
@@ -131,14 +366,117 @@ ensures
       let l1' = !pl1;
       let l2' = !pl2;
       let r = impl_equiv _ l1' _ l2';
-      if (r <> Some false) {
+      if (None? r) {
         pres := r
       } else {
         let n = !pn;
-        let n' : SZ.t = SZ.sub n 1sz;
-        pts_to_serialized_nlist_raw_data_item_head_header' l1' (SZ.v n);
-        pts_to_serialized_nlist_raw_data_item_head_header' l2' (SZ.v n);
-        admit ()
+        with gl1' . assert (pts_to_serialized (serialize_nlist (SZ.v n) serialize_raw_data_item) l1' #p1 gl1');
+        with gl2' . assert (pts_to_serialized (serialize_nlist (SZ.v n) serialize_raw_data_item) l2' #p2 gl2');
+        assume (pure (SZ.fits_u64));
+        raw_data_item_size_eq (List.Tot.hd gl1');
+        raw_data_item_size_eq (List.Tot.hd gl2');
+        if (r = Some true) {
+          let n' = SZ.sub n 1sz;
+          let tl1 = LowParse.Pulse.VCList.nlist_tl
+            serialize_raw_data_item
+            (jump_raw_data_item ())
+            (SZ.v n)
+            l1';
+          Trade.trans _ (pts_to_serialized (serialize_nlist (SZ.v n) serialize_raw_data_item) l1' #p1 gl1') _;
+          pts_to_serialized_nlist_ext
+            serialize_raw_data_item
+            _
+            tl1
+            serialize_raw_data_item
+            (SZ.v n');
+          Trade.trans (pts_to_serialized (serialize_nlist (SZ.v n') serialize_raw_data_item) tl1 #p1 _) _ _;
+          let tl2 = LowParse.Pulse.VCList.nlist_tl
+            serialize_raw_data_item
+            (jump_raw_data_item ())
+            (SZ.v n)
+            l2';
+          Trade.trans _ (pts_to_serialized (serialize_nlist (SZ.v n) serialize_raw_data_item) l2' #p2 gl2') _;
+          pts_to_serialized_nlist_ext
+            serialize_raw_data_item
+            _
+            tl2
+            serialize_raw_data_item
+            (SZ.v n');
+          Trade.trans (pts_to_serialized (serialize_nlist (SZ.v n') serialize_raw_data_item) tl2 #p2 _) _ _;
+          pn := n';
+          pl1 := tl1;
+          pl2 := tl2;
+        } else {
+          let gh1 = pts_to_serialized_nlist_raw_data_item_head_header' l1' (SZ.v n);
+          let (hd1, tl1) = split_nondep_then'
+            _ (jump_header ())
+            _ l1';
+          Trade.trans _ _ (pts_to_serialized (serialize_nlist (SZ.v n) serialize_raw_data_item) l1' #p1 gl1');
+          let h1 = read_header () hd1;
+          Trade.elim_hyp_l _ _ (pts_to_serialized (serialize_nlist (SZ.v n) serialize_raw_data_item) l1' #p1 gl1');
+          rewrite each gh1 as h1;
+          let mt1 = get_header_major_type h1;
+          let gh2 = pts_to_serialized_nlist_raw_data_item_head_header' l2' (SZ.v n);
+          let (hd2, tl2) = split_nondep_then'
+            _ (jump_header ())
+            _ l2';
+          Trade.trans _ _ (pts_to_serialized (serialize_nlist (SZ.v n) serialize_raw_data_item) l2' #p2 gl2');
+          let h2 = read_header () hd2;
+          Trade.elim_hyp_l _ _ (pts_to_serialized (serialize_nlist (SZ.v n) serialize_raw_data_item) l2' #p2 gl2');
+          rewrite each gh2 as h2;
+          let mt2 = get_header_major_type h2;
+          if (mt1 <> mt2) {
+            Trade.elim _ (pts_to_serialized (serialize_nlist (SZ.v n) serialize_raw_data_item) l1' #p1 gl1');
+            Trade.elim _ (pts_to_serialized (serialize_nlist (SZ.v n) serialize_raw_data_item) l2' #p2 gl2');
+            pres := Some false
+          } else {
+            let (lc1, tl1') = split_nondep_then'
+              _ (jump_leaf_content () h1)
+              _ tl1;
+            Trade.trans _ _ (pts_to_serialized (serialize_nlist (SZ.v n) serialize_raw_data_item) l1' #p1 gl1');
+            with w1 . assert (
+              pts_to_serialized (serialize_nondep_then (serialize_nlist (remaining_data_items_header h1) serialize_raw_data_item) (serialize_nlist (SZ.v n - 1) serialize_raw_data_item)) tl1' #p1 w1
+            );
+            list_sum_append raw_data_item_size (fst w1) (snd w1);
+            pts_to_serialized_nlist_append serialize_raw_data_item tl1' _ _;
+            Trade.trans_hyp_r _ _ _ (pts_to_serialized (serialize_nlist (SZ.v n) serialize_raw_data_item) l1' #p1 gl1');
+            pts_to_serialized_length _ tl1';
+            assert (pure (remaining_data_items_header h1 + (SZ.v n - 1) <= SZ.v (S.len tl1')));
+            let n' : SZ.t = SZ.add (impl_remaining_data_items_header (S.len tl1') h1) (SZ.sub n 1sz);
+            pts_to_serialized_nlist_ext
+              serialize_raw_data_item
+              _
+              tl1'
+              serialize_raw_data_item
+              (SZ.v n')
+              ;
+            Trade.trans_hyp_r _ _ _ (pts_to_serialized (serialize_nlist (SZ.v n) serialize_raw_data_item) l1' #p1 gl1');
+
+            let (lc2, tl2') = split_nondep_then'
+              _ (jump_leaf_content () h2)
+              _ tl2;
+            Trade.trans _ _ (pts_to_serialized (serialize_nlist (SZ.v n) serialize_raw_data_item) l2' #p2 gl2');
+            pts_to_serialized_nlist_append serialize_raw_data_item tl2' _ _;
+            Trade.trans_hyp_r _ _ _ (pts_to_serialized (serialize_nlist (SZ.v n) serialize_raw_data_item) l2' #p2 gl2');
+
+            assert (pure (check_equiv_head_correct_pre gl1' gl2' equiv));
+            let sq : squash (check_equiv_head_correct_pre gl1' gl2' equiv) = ();
+            check_equiv_head_correct gl1' gl2' equiv sq;
+            if (impl_check_equiv_head h1 lc1 h2 lc2 (List.Tot.hd gl1') (List.Tot.hd gl2')) {
+                Trade.elim_hyp_l _ _ (pts_to_serialized (serialize_nlist (SZ.v n) serialize_raw_data_item) l1' #p1 gl1');
+                Trade.trans _ (pts_to_serialized (serialize_nlist (SZ.v n) serialize_raw_data_item) l1' #p1 gl1') _;
+                Trade.elim_hyp_l _ _ (pts_to_serialized (serialize_nlist (SZ.v n) serialize_raw_data_item) l2' #p2 gl2');
+                Trade.trans _ (pts_to_serialized (serialize_nlist (SZ.v n) serialize_raw_data_item) l2' #p2 gl2') _;
+                pn := n';
+                pl1 := tl1';
+                pl2 := tl2';
+            } else {
+              Trade.elim _ (pts_to_serialized (serialize_nlist (SZ.v n) serialize_raw_data_item) l1' #p1 gl1');
+              Trade.elim _ (pts_to_serialized (serialize_nlist (SZ.v n) serialize_raw_data_item) l2' #p2 gl2');
+              pres := Some false
+            }
+          }
+        }
       }
     };
     Trade.elim _ (pts_to_serialized (serialize_nlist (SZ.v n1) serialize_raw_data_item) l1 #p1 gl1);
