src/lowparse/pulse/LowParse.Pulse.VCList.fst
@@ -50,6 +50,86 @@ let rec serialize_nlist_append
       (serialize (serialize_nlist n2 s) l2)
   end
 
+ghost
+fn pts_to_serialized_nlist_append
+  (#k: parser_kind)
+  (#t: Type0)
+  (#p: parser k t)
+  (s: serializer p { k.parser_kind_subkind == Some ParserStrong })
+  (x: slice byte)
+  (n1: nat)
+  (n2: nat)
+  (#p: perm)
+  (#v: (nlist n1 t & nlist n2 t))
+requires
+  pts_to_serialized (serialize_nondep_then (serialize_nlist n1 s) (serialize_nlist n2 s)) x #p v
+ensures exists* v' .
+  pts_to_serialized (serialize_nlist (n1 + n2) s) x #p v' **
+  Trade.trade
+    (pts_to_serialized (serialize_nlist (n1 + n2) s) x #p v')
+    (pts_to_serialized (serialize_nondep_then (serialize_nlist n1 s) (serialize_nlist n2 s)) x #p v) **
+  pure (
+    List.Tot.append (fst v) (snd v) == v'
+  )
+{
+  serialize_nondep_then_eq (serialize_nlist n1 s) (serialize_nlist n2 s) v;
+  unfold (pts_to_serialized (serialize_nondep_then (serialize_nlist n1 s) (serialize_nlist n2 s)) x #p v);
+  serialize_nlist_append s n1 (fst v) n2 (snd v);
+  List.Tot.append_length (fst v) (snd v);
+  let v' : nlist (n1 + n2) t = List.Tot.append (fst v) (snd v);
+  fold (pts_to_serialized (serialize_nlist (n1 + n2) s) x #p v');
+  intro
+    (Trade.trade
+      (pts_to_serialized (serialize_nlist (n1 + n2) s) x #p v')
+      (pts_to_serialized (serialize_nondep_then (serialize_nlist n1 s) (serialize_nlist n2 s)) x #p v)
+    )
+    fn _ {
+      unfold (pts_to_serialized (serialize_nlist (n1 + n2) s) x #p v');
+      fold (pts_to_serialized (serialize_nondep_then (serialize_nlist n1 s) (serialize_nlist n2 s)) x #p v);
+    }
+}
+
+ghost
+fn pts_to_serialized_nlist_ext
+  (#k1: parser_kind)
+  (#t1: Type0)
+  (#p1: parser k1 t1)
+  (s1: serializer p1 { k1.parser_kind_subkind == Some ParserStrong })
+  (n1: nat)
+  (x: slice byte)
+  (#k2: parser_kind)
+  (#t2: Type0)
+  (#p2: parser k2 t2)
+  (s2: serializer p2 { k2.parser_kind_subkind == Some ParserStrong })
+  (n2: nat)
+  (#p: perm)
+  (#v1: nlist n1 t1)
+requires
+  pts_to_serialized (serialize_nlist n1 s1) x #p v1 **
+  pure (t1 == t2) **
+  pure (
+    t1 == t2 /\
+    (forall b . parse p1 b == parse p2 b)
+  ) **
+  pure (n1 == n2)
+ensures exists* v2 .
+  pts_to_serialized (serialize_nlist n2 s2) x #p v2 **
+  Trade.trade
+    (pts_to_serialized (serialize_nlist n2 s2) x #p v2)
+    (pts_to_serialized (serialize_nlist n1 s1) x #p v1) **
+  pure (
+    t1 == t2 /\
+    n1 == n2 /\
+    (v1 <: list t1) == v2
+  )
+{
+  parse_nlist_ext_forall n1 p1 p2;
+  pts_to_serialized_ext_trade
+    (serialize_nlist n1 s1)
+    (serialize_nlist n2 s2)
+    x;
+}
+
 inline_for_extraction
 fn jump_nlist
    (#t: Type0)
